rm old file in meta

state/TargetLangIFC.fst
@@ -186,12 +186,12 @@ let elab_typ (t:typ) : Type =
 let elab_typ_tgt (t:typ) : witnessable (elab_typ t)=
   dsnd (_elab_typ t inv_low_contains)
 
-let eliminate_inv_low (h:lheap) (a:typ) (r:ref (elab_typ a)) :
+let eliminate_inv_low (h:lheap) (a:typ) #inv (r:ref (dfst (_elab_typ a inv))) :
   Lemma
     (requires (inv_low_points_to_low h))
     (ensures (
-        (witnessable_ref (elab_typ a) #(elab_typ_tgt a)).satisfy r h is_low_pred ==> 
-          (elab_typ_tgt a).satisfy (sel h r) h is_low_pred
+        (witnessable_ref (dfst (_elab_typ a inv)) #(dsnd (_elab_typ a inv))).satisfy r h is_low_pred ==> 
+          (dsnd (_elab_typ a inv)).satisfy (sel h r) h is_low_pred
     )) = ()
 
 let eliminate_inv_contains (h:lheap) (a:typ) (r:ref (elab_typ a)) :
@@ -222,11 +222,34 @@ let write' (#t:Type) {| c:witnessable t |} (r:ref t) (v:t)
     modifies_only_label Low h0 h1 /\
     shallowly_contained_low r h1))
 = let h0 = get () in
-  r := v;
+  write r v;
   let h1 = get () in
-  assume (inv_low_points_to_low h1);
+  introduce 
+  forall (a:typ) (inv:lheap -> Type0).
+    let tt = _elab_typ a inv in
+    forall (r:ref (dfst tt)).
+      (witnessable_ref (dfst tt) #(dsnd tt)).satisfy r h1 is_low_pred ==> 
+        (dsnd tt).satisfy (sel h1 r) h1 is_low_pred
+  with begin
+    let tt = _elab_typ a inv in
+    introduce forall (r:ref (dfst tt)).
+      (witnessable_ref (dfst tt) #(dsnd tt)).satisfy r h1 is_low_pred ==> 
+        (dsnd tt).satisfy (sel h1 r) h1 is_low_pred
+    with begin
+      introduce (witnessable_ref (dfst tt) #(dsnd tt)).satisfy r h1 is_low_pred 
+        ==> (dsnd tt).satisfy (sel h1 r) h1 is_low_pred
+      with _. begin
+        introduce (dsnd tt).satisfy (sel h0 r) h0 is_low_pred ==> 
+          (dsnd tt).satisfy (sel h1 r) h1 is_low_pred with _. eliminate_inv_low h0 a #inv r;
+        admit ()
+      end
+    end
+  end;
+  assert (inv_low_points_to_low h1);
   assume (inv_contains_points_to_contains h1);
   ()
+
+let _ = assert False
 
 let _alloc (#a:Type) (init:a)
 : IST (ref a) (fun h -> True) (alloc_post #a init)
